theories/Pipeline.v
@@ -120,10 +120,11 @@ Definition compile_pir_directly (p : Ast.Env.program) (dearg : bool) :=
 (* Eval cbv in compile_pir_directly <# gal_id #> false. *)
 
 Definition translatable_program (p : Ast.Env.program) : Prop :=
-  exists epT, translate_program p = epT.
+  exists eΣ ann_env init, translate_program p false = ((eΣ; ann_env), init).
 
 Definition translatable_typed_eprogram (epT : typed_eprogram) : Prop :=
-  let '((eΣ; ann_env), init) := epT in ProgramInSubset eΣ init.
+  let '((eΣ; ann_env), init) := epT in ProgramInSubset eΣ init /\
+    env_annots_sensible remap_env pir_ignore_default eΣ ann_env.
 
 Definition pir_fuel := 5000.
 Definition pir_program := (unit * term).
@@ -151,8 +152,12 @@ Program Definition gallina_to_lbt_transform :
      preservation _ _ _ _ := _
   |}.
 Next Obligation.
-(* Needs subset & well-typed precondition *)
-Admitted. 
+  eexists. split; [|trivial].
+  destruct p as [pΣ t].
+  inversion e. simpl in X.
+  inversion X; subst; hnf; try eauto; admit.
+(* needs subset & well-typed precondition *)
+Admitted.
 
 Program Definition lbt_to_pir_transform :
   Transform.t (∑ env : ExAst.global_env, env_annots box_type env) unit kername term EAst.term term
@@ -173,9 +178,9 @@ Next Obligation.
   unfold eval_pir_program.
   unfold translatable_typed_eprogram in *.
   destruct p as [[eΣ ann_env] kn].
-  destruct e.
+  destruct t1 as [Hsub Henv]. destruct e. destruct Hsub as [Hall_sub [cb Hdecl]].
   destruct (lookup_constant_body eΣ kn) eqn:Hlookup; try discriminate.
-  simpl in H. destruct t1 as [Hall_sub [cb Hdecl]].
+  simpl in H.
   (* apply (subset_is_translatable remap_env) in t1 as Htl.
   destruct Htl as [ann_t [t' tl]]. simpl in H.
   evar (ann_v : annots box_type t0).
@@ -202,28 +207,3 @@ Definition compile_and_print_pir (p : Ast.Env.program) :=
 
 (* Eval vm_compute in <# fun b : bool => b #>.
 Eval vm_compute in compile_and_print_pir <# gal_id #>. *)
-
-Section Test.
-
-Variable (Σ  : Env.global_env).
-Variable (t  : Ast.term).
-
-Variable (eΣ  : ExAst.global_env).
-Variable (et : EAst.term).
-
-Variable (t' : PIR.term).
-
-Variable (sub : InSubset eΣ [] et).
-
-Lemma precond : pre gallina_to_lbt_transform (Σ, t).
-Proof.
-  hnf. easy.
-Qed.
-
-Definition test := sub.
-
-End Test.
-
-(* Require Import MetaCoq.ErasurePlugin.ErasureCorrectness.
-
-Check @verified_erasure_pipeline_theorem. *)
